Add (partial )solution to HumanEval160

HumanEvalLean/HumanEval160.lean
@@ -1,5 +1,118 @@
-def do_algebra : Unit :=
-  ()
+inductive Op where
+  | add
+  | sub
+  | mul
+  | div
+  | pow
+
+namespace Op
+
+instance : ToString Op where
+  toString
+    | add => "+"
+    | sub => "-"
+    | mul => "*"
+    | div => "/"
+    | pow => "^"
+
+def prio : Op → Nat
+  | add | sub => 1
+  | mul | div => 2
+  | pow       => 3
+
+def leftAssoc : Op → Bool
+  | add | sub => true
+  | mul | div => true
+  | pow       => false
+
+def interpret : Op → (Nat → Nat → Nat)
+  | add => (· + ·)
+  | sub => (· - ·)
+  | mul => (· * ·)
+  | div => (· / ·)
+  | pow => (· ^ ·)
+
+end Op
+
+inductive Expr where
+  | lit (n : Nat)
+  | app (op : Op) (arg₁ arg₂ : Expr)
+  deriving Inhabited
+
+namespace Expr
+
+instance : ToString Expr where
+  toString :=
+    let rec go
+      | .lit n            => s!"{n}"
+      | .app op arg₁ arg₂ => s!"({go arg₁} {op} {go arg₂})"
+    go
+
+def eval : Expr → Nat
+  | lit n            => n
+  | app op arg₁ arg₂ => op.interpret arg₁.eval arg₂.eval
+
+structure ParseState where
+  ops    : List Op   := []
+  args   : List Nat  := []
+  hold   : List Op   := []
+  output : List Expr := []
+  deriving Inhabited
+
+namespace ParseState
+
+def pushArg (σ : ParseState) (arg : Nat) : ParseState :=
+  { σ with output := (lit arg) :: σ.output }
+
+@[simp]
+theorem pushArg_ops (σ : ParseState) : (σ.pushArg arg).ops = σ.ops := rfl
+
+def pushOp (σ : ParseState) (op : Op) : ParseState :=
+  match σ.hold with
+  | [] => { σ with hold := [op] }
+  | top :: hold =>
+    match compare top.prio op.prio, top.leftAssoc with
+    | .lt, _ | .eq, false => { σ with hold := op :: top :: hold }
+    | .gt, _ | .eq, true =>
+      match σ.output with
+      | arg₂ :: arg₁ :: out => { σ with hold := op :: hold, output := .app top arg₁ arg₂ :: out }
+      | _                   => σ -- Trash value chosen to easily satisfy `pushOp_ops`.
+
+@[simp]
+theorem pushOp_ops (σ : ParseState) : (σ.pushOp op).ops = σ.ops := by
+  rw [pushOp]
+  repeat (split <;> try rfl)
+
+def finalize (σ : ParseState) : ParseState :=
+  match _ : σ.hold, σ.output with
+  | op :: hold, arg₂ :: arg₁ :: out => finalize { σ with hold, output := .app op arg₁ arg₂ :: out }
+  | _, _                            => σ
+  termination_by σ.hold
+  decreasing_by simp_all +arith
+
+end ParseState
+
+-- Parses an expression based on the "shunting yard algorithm".
+def parse! (ops : List Op) (args : List Nat) : Expr :=
+  go { ops, args } |>.output[0]!
+where
+  go (σ : ParseState) : ParseState :=
+    match _ : σ.ops, σ.args with
+    | op :: ops, arg :: args => { σ with ops, args }  |>.pushArg arg |>.pushOp op |> go
+    | [],        [arg]       => { σ with args := [] } |>.pushArg arg |>.finalize
+    | _,         _           => panic! "Invalid parse state"
+  termination_by σ.ops
+  decreasing_by simp_all +arith
+
+end Expr
+
+def doAlgebra (ops : List Op) (args : List Nat) : Nat :=
+  Expr.parse! ops args |>.eval
+
+example : doAlgebra [.add, .mul, .sub] [2, 3, 4, 5] = 9  := by native_decide
+example : doAlgebra [.pow, .mul, .add] [2, 3, 4, 5] = 37 := by native_decide
+example : doAlgebra [.add, .mul, .sub] [2, 3, 4, 5] = 9  := by native_decide
+example : doAlgebra [.div, .mul]       [7, 3, 4]    = 8  := by native_decide
 
 /-!
 ## Prompt
@@ -8,16 +121,16 @@ def do_algebra : Unit :=
 
 def do_algebra(operator, operand):
     """
-    Given two lists operator, and operand. The first list has basic algebra operations, and 
-    the second list is a list of integers. Use the two given lists to build the algebric 
+    Given two lists operator, and operand. The first list has basic algebra operations, and
+    the second list is a list of integers. Use the two given lists to build the algebric
     expression and return the evaluation of this expression.
 
     The basic algebra operations:
-    Addition ( + ) 
-    Subtraction ( - ) 
-    Multiplication ( * ) 
-    Floor division ( // ) 
-    Exponentiation ( ** ) 
+    Addition ( + )
+    Subtraction ( - )
+    Multiplication ( * )
+    Floor division ( // )
+    Exponentiation ( ** )
 
     Example:
     operator['+', '*', '-']
